src/CompilationUnit.v
@@ -1,0 +1,11 @@
+Require Import List HList SourceLang.
+Import ListNotations.
+
+Record compilation_unit :=
+  CompilationUnit {
+      types : list type;
+      exprs : hlist (expr []) types
+  }.
+
+Definition singleton {ty} (e : expr [] ty) : compilation_unit := 
+  CompilationUnit [ty] (hcons e hnil).
